Common.v
@@ -17,7 +17,7 @@ Fixpoint replicate {A : Set} (n : nat) (a : A) :=
 Lemma replicate_app : forall {A : Set} (n m : nat) (a : A),
   replicate n a ++ replicate m a = replicate (n + m) a.
   intros.
-  by induction n ; last (simpl ; f_equal).
+  by induction n ; last simpl ; f_equal.
 Qed.
 
 Lemma replicate_rev_id :
@@ -34,7 +34,7 @@ Qed.
 rt1n_trans:
   clos_refl_trans_1n は推移関係である。
 *)
-Theorem rt1n_trans' : forall (A : Type) (R : relation A) (x y z : A),
+Lemma rt1n_trans' : forall (A : Type) (R : relation A) (x y z : A),
   clos_refl_trans_1n A R x y -> clos_refl_trans_1n A R y z ->
   clos_refl_trans_1n A R x z.
   intros.
